

N1.

$$\begin{aligned}
 I_n(\alpha) &= \int_0^1 \frac{x^n}{x+\alpha} dx = \int_0^1 \frac{x^{n-1} \cdot x}{x+\alpha} dx = \\
 &= \int_0^1 \frac{x^{n-1} (x-\alpha+\alpha)}{x+\alpha} dx = \int_0^1 x^{n-1} dx - \int_0^1 \frac{\alpha x^{n-1}}{x+\alpha} dx = \frac{1}{n} x^n \Big|_0^1 - \\
 &\quad - \alpha \int_0^1 \frac{x^{n-1}}{x+\alpha} dx
 \end{aligned}$$

$$\boxed{I_n(\alpha) = \frac{1}{n} - \alpha I_{n-1}} \quad \leftarrow \text{формула}$$

$$\begin{aligned}
 I_0(\alpha) &= \int_0^1 \frac{x^0}{x+\alpha} dx = \int_0^1 \frac{dx}{x+\alpha} = \ln|x+\alpha| \Big|_0^1 = \\
 &= \ln|1+\alpha| - \ln|\alpha| = \ln \left| \frac{1+\alpha}{\alpha} \right|
 \end{aligned}$$

Обратная рекурсия:

$$I_n(\alpha) = \frac{1}{n} - \alpha I_{n-1}$$

$$I_{n-1} = \frac{1}{n\alpha} - \frac{I_n(\alpha)}{\alpha}$$

$$\boxed{I_n = \frac{1}{\alpha(n+1)} - \frac{I_{n+1}(\alpha)}{\alpha}} \quad \leftarrow \text{формула}$$

№3.

$$a_0 = 1, a_1 = -3$$

$$a_n = 6a_{n-2} - a_{n-1}$$

Предположим $a_n = 2^n$, тогда:

$$2^{\frac{3}{2}} = 6 \cdot \frac{1}{2^2} - \frac{2^{\frac{1}{2}}}{2}$$

\Downarrow

$$2^2 + 2 - 6 = 0$$

\Downarrow

$$\begin{cases} 2 = 2 \\ 2 = -3 \end{cases}$$

$$a_n = \alpha 2^n + \beta (-3)^n$$

$$\text{Найдём } \alpha, \beta = \text{const: } \begin{cases} \alpha + \beta = a_0 \\ 2\alpha - 3\beta = a_1 \end{cases} \Rightarrow \begin{cases} \alpha + \beta = 1 \\ 2\alpha - 3\beta = -3 \end{cases} \Rightarrow \begin{cases} \alpha = 0 \\ \beta = 1 \end{cases}$$

$$a_{2020} = (-3)^{2020} = \boxed{3^{2020}}$$

1/4.

$$A = \begin{pmatrix} 1 & 10 \\ s & 1 \end{pmatrix}, \quad \varepsilon(s) = \max \lambda(\phi), \quad s > 0$$

$$k(s) = ? \quad (s = 10 \text{ и } s = 0,1)$$

Решение:

$$\det(A - \lambda I) = \begin{vmatrix} 1-\lambda & 10 \\ s & 1-\lambda \end{vmatrix} = (1-\lambda)^2 - 10s = 0$$

\Downarrow

$$1 - 2\lambda + \lambda^2 - 10s = 0$$

$$\lambda^2 - 2\lambda + (1 - 10s) = 0$$

$$D = 4 - 4(1 - 10s)$$

$$\lambda_{1,2} = \frac{2 \pm \sqrt{40s}}{2} = 1 \pm \sqrt{10s}$$

$$\lambda_{\max} = 1 + \sqrt{10s}$$

$$k(s) = \frac{d\varepsilon(s)}{ds} = \frac{\sqrt{10}}{2} \cdot \frac{1}{\sqrt{s}} = \frac{\sqrt{10}}{2} \cdot s^{-\frac{1}{2}}$$

$$k(s=10) = \frac{\sqrt{10}}{2} \cdot \frac{1}{\sqrt{10}} = \boxed{\frac{1}{2}}$$

$$k(s=0,1) = \frac{\sqrt{10}}{2} \cdot \frac{1}{\sqrt{\frac{1}{10}}} = \frac{10}{2} = \boxed{5}$$